DDC/src/grade.v
@@ -9,6 +9,10 @@ Require Export Qual.subst.
 Set Implicit Arguments.
 Open Scope grade_scope.
 
+Ltac invert_CGrade a :=
+  match goal with 
+    [ H : CGrade ?P ?phi ?psi a |- _] => inversion H ; subst 
+  end.
 
 Lemma Step_Grade : forall a b,  Step a b -> forall P phi, Grade P phi a -> Grade P phi b.
 Proof.
@@ -22,18 +26,17 @@ Proof.
   - (* Beta / AppRel *)
     invert_Grade; subst.
     pick fresh x;  spec x.
+    invert_CGrade b; auto.
     eapply Grade_open; eauto.
-  - (* Beta / AppIrrel *)
-    invert_Grade; subst.
-    pick fresh x;  spec x.
     eapply Grade_open_irrel; eauto.
   - (* SPair *)
-   invert_Grade; subst; eauto; try done.
+   invert_Grade; invert_CGrade a1; subst; eauto; try done.
   - (* LetPair *)
     invert_Grade; subst;
     pick fresh x; spec x.
-    eapply G_AppRel; eauto using leq_Bot.
+    eapply G_App; eauto using leq_Bot.
+    invert_CGrade a1.
     eapply Grade_open; eauto.
-    eapply G_AppRel; eauto using leq_Bot.
     eapply Grade_open_irrel; eauto. 
 Qed.
+
