DDC/src/sort_sig.v
@@ -1,0 +1,9 @@
+Parameter sort : Set.
+Parameter axiom : sort -> sort -> Prop.
+Parameter rule : sort -> sort -> sort -> Prop.
+
+Parameter star : sort.
+
+Definition size_sort (s:sort) := 1.
+
+Parameter sort_regularity : forall s1, exists s2, axiom s1 s2.
